coq/theories/functional/FunValues.v
@@ -1,7 +1,0 @@
-Module FunValues.
-
-Inductive Value :=
-  | Pair (v1 v2 : Value)
-  | Num (n : nat).
-
-End FunValues.
