coq/TODOs.md
@@ -1,0 +1,8 @@
+TODO:
+- llist
+- word4
+- termination of c_cmd
+- Alias that isn't substituted everywhere? `name := nat` (not Notation)
+
+Done?:
+- char – used Coq.Strings.Ascii.ascii
